theories/exn.v
@@ -1,0 +1,61 @@
+From stdpp Require Import base option.
+
+Set Universe Polymorphism.
+
+Section exceptions.
+  Variables (E: Type).
+
+  Inductive exn (A : Type) : Type := 
+  | Err (e: E)
+  | OK (a: A).
+  Arguments Err {A} e.
+  Arguments OK {A} a.
+  
+  Definition exn_to_opt {A: Type} (c: exn A) : option A :=
+    match c with
+    | Err _ => None
+    | OK a => Some a
+    end.
+
+  Definition exn_map {A B: Type} (f: A -> B) (c: exn A) : exn B :=
+    match c with
+    | Err e => Err e
+    | OK a => OK (f a)
+    end.
+
+  Definition exn_bind {A B: Type} (f: A -> exn B) (c: exn A) : exn B :=
+    match c with
+    | Err e => Err e
+    | OK a => f a
+    end.
+
+  Definition exn_join {A: Type} (c: exn (exn A)) : exn A :=
+    match c with
+    | OK (OK a) => OK a
+    | OK (Err e)
+    | Err e => Err e
+    end.
+
+End exceptions.
+
+
+#[export]
+Instance exn_FMap {E} : FMap (exn E) := @exn_map E.
+
+#[export]
+Instance exn_MBind {E} : MBind (exn E) := @exn_bind E.
+
+#[export]
+Instance exn_MRet {E} : MRet (exn E) := @OK E.
+
+#[export]
+Instance exn_MJoin {E} : MJoin (exn E) := @exn_join E.
+
+#[export]
+Instance exn_throw {E} : MThrow E (exn E) := @Err E.
+
+Definition guard_opt {E A} (err: E) (c: option A) : exn E A :=
+  match c with
+  | Some a => mret a
+  | None => mthrow err
+  end.
